added predicates & corrections

BPTNode.dfy
@@ -1,6 +1,6 @@
 
 class BPTNode {
-    
+    const ORDER := 5
     // array of length ORDER
     var keys: array<int>
     // array of length ORDER + 1
@@ -17,43 +17,74 @@ class BPTNode {
     ghost var Repr: set<BPTNode>
 
 
-// #### For all nodes 
-// - min_keys : must contain at least floor(n/2) keys.
+    // ################ For all nodes ################
+    // - min_keys : must contain at least floor(n/2) keys.
+    
+    ghost predicate sorted()
+        //keys are sorted from left two right
+        reads this, keys, children
+        requires length_ok()
+    {
+        forall i: int :: 0 <= i < keynum-1 ==> (
+            keys[i] < keys[i+1]
+        )
+    }
 
-    // #### For internal nodes
+
+    // ################ For internal nodes ################
     ghost predicate child_nb()
         // contains one more child than it has keys. 
         reads this, keys, children
-        requires is_leaf==false
         requires length_ok()
     {
-        (forall i: int :: 0 <= i < keynum ==> (
-            keys[i] > 0 && 
-            children[i] is BPTNode
-        )) &&
-        children[keynum] is BPTNode
-        // why ?
+        is_leaf==false ==> (
+            (forall i: int :: 0 <= i < keynum ==> (
+                keys[i] > 0 && 
+                children[i] is BPTNode
+            )) &&
+            children[keynum] is BPTNode
+        )
     }
 
 
     ghost predicate child_height_eq()
+        // all subtrees must be the same height. 
         reads *
         requires is_leaf==false
         requires length_ok()
         requires child_nb()
     {   
-        (forall i: int :: 0 <= i < keynum ==> (
+        (forall i: int :: 0 <= i < keynum+1 ==> (
             children[i].height == height -1
         ))
     }
-// all subtrees must be the same height. 
-// - hierarchy : all keys in a given subtree is bounded by surrounding keys in parent node.
-// 
-// #### for leaves
-// - leaves_height_eq : all leaves are at the same distance from the root (always -1).
-// - linked_leaves : contains extra pointer towards the next leaf.
-// - sorted : keys are sorted from left two right
-// - all_keys_in_leaves : all keys appear in a leaf node.
+    
+    ghost predicate hierarchy()
+        // all keys in a given subtree is bounded by surrounding keys in parent node.
+        reads * 
+        requires is_leaf==false
+        requires length_ok()
+        requires child_nb()
+    {
+        forall i: int :: 0 <= i < keynum+1 ==> (
+            (forall k :: k in children[i].Contents ==> (
+                (i > 0 ==> k >= keys[i-1]) &&
+                (i< keynum ==> k <= keys[i])
+            ))
+        )
+    }
+
+    // ################ for leaves ################
+    ghost predicate leaves_height_eq()
+        // all leaves are at the same distance from the root (always -1).
+        reads this
+    {
+        is_leaf <==> height==-1
+    }
+
+
+    // - linked_leaves : contains extra pointer towards the next leaf.
+    // - all_keys_in_leaves : all keys appear in a leaf node.
 
     ghost predicate length_ok()
         // the keys and children array are well formed
@@ -61,7 +92,8 @@ class BPTNode {
     {
         keys.Length == ORDER &&
         children.Length == ORDER+1 &&
-        keynum <= ORDER
+        keynum < ORDER + 1 &&
+        keynum >= 0 
     }
 
     ghost predicate empty()
